## Lead Up
Consider a [[Groups|group]] $C_{2}$ with two elements ([[Cyclic Groups|$\cong \mathbb{Z} /2$]]) , say $C_{2}=\left\{ \pm 1 \right\}$ with $1=e$, then consider the [[Functions|map]] [[Symmetric Groups|$S_{n}\to C_{2}$]] given by $\sigma \mapsto \text{sgn}(\sigma)$
### Lemma
The map $\text{sgn}:S_{n}\to C_{2}$ with $\sigma \mapsto \text{sgn}(\sigma)$ is a [[Homomorphisms|homomorphism]] of groups
#### Proof
We need $\text{sgn}(\sigma_{1})\text{sgn}(\sigma_{2})=\text{sgn}(\sigma_{1}\sigma_{2})$ which follows from [[Inversion of Permutation#Corollary|this corollary]] because we can count the number of transpositions
## Definition
We define the alternating group $A_{n}$ of all even permutations in $S_{n}$, so 
$$
A_{n}=\text{ker}(\text{sgn})=\left\{ \sigma \in S_{n}|\text{sgn}(\sigma)=+1 \right\}
$$
So $\sigma$ is the product of an even number of permutations, in the [[Symmetric Groups|symmetric group]]. 
## Lemma
- $\left| A_{n} \right|=\frac{n!}{2}$
- The alternating group is a [[Subgroups|subgroup]] of the symmetric group, in fact [[Normal Subgroups|$A_{n} \lhd S_{n}$]] 
- $A_{n}$ is generated by 3-cycles
### Proof
Since $\text{sgn}:S_{n}\to C_{2}$, $\text{ker}(\text{sgn})=A_{n},\text{im}(\text{sgn})=C_{2}$, then by the [[First Isomorphism Theorem|first isomorphism theorem]],
$$
S_{n} /A_{n}\cong C_{2}
$$
By some lemma, $\left| C_{2} \right|=\frac{\left| S_{n} \right|}{\left| A_{n} \right|}\implies \left| A_{n} \right|=\frac{n!}{2}$
___
Since $A_{n}=\text{ker}(\text{sgn}:S_{n}\to C_{2})$, by some lemma, every kernel of a homomorphism is is a normal subgroup
___
left as exercise
## Example
$$
A_{3}=\left\{ e,\begin{pmatrix}
1 & 2 & 3
\end{pmatrix},\begin{pmatrix}
3 & 2 & 1
\end{pmatrix} \right\}
$$
___
We know $A_{4}$ is also made up of 3-cycles, and $\left| A_{4} \right|=12$. We can work out how many 3-cycles there are, in the first position of the 3-cycle, there are $\hspace{0pt}4$ options, in the second, there are $\hspace{0pt}3$ options left and finally the third would have $\hspace{0pt}2$ choices, so we have $\hspace{0pt}24$ total 3-cycles. But we also know that 3-cycles are rotationally symmetric, i.e. $\begin{pmatrix}a & b & c \end{pmatrix}=\begin{pmatrix}c & a & b \end{pmatrix}=\begin{pmatrix}b & c & a\end{pmatrix}$, so we can divide this number of 3-cycles by $\hspace{0pt}3$, getting $\hspace{0pt}8$ of them, to fill the remaining elements, we need to consider the final transpositions we have left, which can be written as a product of 3-cycles e.g.
$$
\begin{pmatrix}
1 & 2
\end{pmatrix}\begin{pmatrix}
3 & 4
\end{pmatrix}=\begin{pmatrix}
1 & 2 
\end{pmatrix}\begin{pmatrix}
2 & 3
\end{pmatrix}\begin{pmatrix}
2 & 3
\end{pmatrix}\begin{pmatrix}
3 & 4
\end{pmatrix}=\begin{pmatrix}
1 & 2 & 3
\end{pmatrix}\begin{pmatrix}
2 & 3 & 4
\end{pmatrix}
$$
So
$$
A_{4}=\left\{ e, 3\text{-cycles},\begin{pmatrix}
1 & 2
\end{pmatrix}\begin{pmatrix}
3 & 4
\end{pmatrix},\begin{pmatrix}
1 & 3
\end{pmatrix}\begin{pmatrix}
2 & 4
\end{pmatrix},\begin{pmatrix}
1 & 4 
\end{pmatrix}\begin{pmatrix}
2 & 3
\end{pmatrix} \right\}
$$

